tests/elab/bv_extract.lean
@@ -20,7 +20,8 @@ theorem bv_ofBool_1 (h : x = 1#64) : ofBool (x.getLsbD 0) = 1#1 := by
 theorem bv_ofBool_2 (h : x = 1#64) : ofBool (x.getLsbD 1) = 0#1 := by
   bv_decide
 
-set_option maxHeartbeats 10000000000 in
+set_option trace.Meta.Tactic.cbv true
+set_option maxHeartbeats 10000000 in
 theorem bv_ofBool_3 (h : x = 1#1) : ofBool x[0] = 1#1 := by
   bv_decide +showCbvGoal
   cbv
